Update certicoq vanilla plugin w/ primitive floats

cplugin/.Makefile.d
@@ -1,3 +1,15 @@
-CertiCoqVanilla.vo CertiCoqVanilla.glob CertiCoqVanilla.v.beautified CertiCoqVanilla.required_vo: CertiCoqVanilla.v ./certicoq_vanilla_plugin$(DYNOBJ)
-CertiCoqVanilla.vio: CertiCoqVanilla.v ./certicoq_vanilla_plugin$(DYNOBJ)
-CertiCoqVanilla.vos CertiCoqVanilla.vok CertiCoqVanilla.required_vos: CertiCoqVanilla.v ./certicoq_vanilla_plugin$(DYNOBJ)
+Loader.vo Loader.glob Loader.v.beautified Loader.required_vo: Loader.v ./certicoq_vanilla_plugin$(DYNOBJ)
+Loader.vio: Loader.v ./certicoq_vanilla_plugin$(DYNOBJ)
+Loader.vos Loader.vok Loader.required_vos: Loader.v ./certicoq_vanilla_plugin$(DYNOBJ)
+CoqMsgFFI.vo CoqMsgFFI.glob CoqMsgFFI.v.beautified CoqMsgFFI.required_vo: CoqMsgFFI.v Loader.vo
+CoqMsgFFI.vio: CoqMsgFFI.v Loader.vio
+CoqMsgFFI.vos CoqMsgFFI.vok CoqMsgFFI.required_vos: CoqMsgFFI.v Loader.vos
+PrimInt63.vo PrimInt63.glob PrimInt63.v.beautified PrimInt63.required_vo: PrimInt63.v Loader.vo
+PrimInt63.vio: PrimInt63.v Loader.vio
+PrimInt63.vos PrimInt63.vok PrimInt63.required_vos: PrimInt63.v Loader.vos
+PrimFloats.vo PrimFloats.glob PrimFloats.v.beautified PrimFloats.required_vo: PrimFloats.v Loader.vo
+PrimFloats.vio: PrimFloats.v Loader.vio
+PrimFloats.vos PrimFloats.vok PrimFloats.required_vos: PrimFloats.v Loader.vos
+CertiCoqVanilla.vo CertiCoqVanilla.glob CertiCoqVanilla.v.beautified CertiCoqVanilla.required_vo: CertiCoqVanilla.v Loader.vo CoqMsgFFI.vo PrimInt63.vo PrimFloats.vo
+CertiCoqVanilla.vio: CertiCoqVanilla.v Loader.vio CoqMsgFFI.vio PrimInt63.vio PrimFloats.vio
+CertiCoqVanilla.vos CertiCoqVanilla.vok CertiCoqVanilla.required_vos: CertiCoqVanilla.v Loader.vos CoqMsgFFI.vos PrimInt63.vos PrimFloats.vos
