cplugin/runtime/coq_c_ffi.h
@@ -1,0 +1,5 @@
+#include "values.h"
+
+extern value coq_msg_debug(value msg);
+extern value coq_msg_info(value msg);
+extern value coq_user_error(value msg);
