plugin/static/printCsyntax.ml
@@ -478,8 +478,8 @@ let print_init p = function
   | Init_int16 n -> fprintf p "%ld" (camlint_of_coqint n)
   | Init_int32 n -> fprintf p "%ld" (camlint_of_coqint n)
   | Init_int64 n -> fprintf p "%LdLL" (camlint64_of_coqint n)
-  | Init_float32 n -> fprintf p "%.15F" (camlfloat_of_coqfloat n)
-  | Init_float64 n -> fprintf p "%.15F" (camlfloat_of_coqfloat n)
+  | Init_float32 n -> print_float p "%.15F" (camlfloat_of_coqfloat n)
+  | Init_float64 n -> print_float p "%.15F" (camlfloat_of_coqfloat n)
   | Init_space n -> fprintf p "/* skip %s */@ " (Z.to_string n)
   | Init_addrof(symb, ofs) ->
       let ofs = camlint_of_coqint ofs in
