bootstrap/certicoqc/Loader.v
@@ -1,4 +1,5 @@
 From MetaCoq.Template Require Import ExtractableLoader.
-From CertiCoq Require Import CertiCoqVanilla. (* We reuse the ML certicoq plugin to parse options and print Clight code *)
+From CertiCoq Require Export CertiCoqVanilla. (* We reuse the ML certicoq plugin to parse options and print Clight code *)
+(* Use Export to export the primitives registrations *)
 
 Declare ML Module "certicoqc_plugin".
