cplugin/CertiCoqVanilla.v
@@ -1,5 +1,2 @@
-Require Import String.
-From MetaCoq.Template Require Import All.
-
-Declare ML Module "metacoq_template_plugin".
-Declare ML Module "certicoq_vanilla_plugin".
+From CertiCoq.VanillaPlugin Require Import Loader.
+From CertiCoq.VanillaPlugin Require Export CoqMsgFFI PrimInt63 PrimFloats.
